pairing heap: start adding parent relation

Weidenbach_Book/IsaSAT/Inplace_Pairing_Heaps.thy
@@ -10,57 +10,112 @@ text \<open>In this section, we replace the tree version by several arrays that 
   the relations (parent, child, next, previous) of the same trees.\<close>
 
 (*TODO: this is missing the parents*)
-type_synonym ('a, 'b) hp_fun = \<open>(('a \<Rightarrow> 'a option) \<times> ('a \<Rightarrow> 'a option) \<times> ('a \<Rightarrow> 'a option) \<times> ('a \<Rightarrow> 'b option))\<close>
+type_synonym ('a, 'b) hp_fun = \<open>(('a \<Rightarrow> 'a option) \<times> ('a \<Rightarrow> 'a option) \<times> ('a \<Rightarrow> 'a option) \<times> ('a \<Rightarrow> 'a option) \<times> ('a \<Rightarrow> 'b option))\<close>
 
-definition hp_set_all :: \<open>'a \<Rightarrow> 'a option \<Rightarrow> 'a option \<Rightarrow> 'a option \<Rightarrow> 'b option  \<Rightarrow> ('a, 'b) hp_fun  \<Rightarrow> ('a, 'b) hp_fun \<close> where
-  \<open>hp_set_all i prev nxt child sc = (\<lambda>(prevs, nxts, childs, scores). (prevs(i:=prev), nxts(i:=nxt), childs(i:=child), scores(i:=sc)))\<close>
+definition hp_set_all :: \<open>'a \<Rightarrow> 'a option \<Rightarrow> 'a option \<Rightarrow> 'a option \<Rightarrow> 'a option \<Rightarrow> 'b option  \<Rightarrow> ('a, 'b) hp_fun \<Rightarrow> ('a, 'b) hp_fun \<close> where
+  \<open>hp_set_all i prev nxt child par sc = (\<lambda>(prevs, nxts, childs, parents, scores). (prevs(i:=prev), nxts(i:=nxt), childs(i:=child), parents(i:=par), scores(i:=sc)))\<close>
 
 
 definition hp_update_prev :: \<open>'a \<Rightarrow> 'a option \<Rightarrow> ('a, 'b) hp_fun \<Rightarrow> ('a, 'b) hp_fun\<close> where
-  \<open>hp_update_prev i prev = (\<lambda>(prevs, nxts, childs, scores). (prevs(i:=prev), nxts, childs, scores))\<close>
+  \<open>hp_update_prev i prev = (\<lambda>(prevs, nxts, childs, parents, score). (prevs(i:=prev), nxts, childs, parents, score))\<close>
 
 definition hp_update_nxt :: \<open>'a \<Rightarrow> 'a option \<Rightarrow> ('a, 'b) hp_fun \<Rightarrow> ('a, 'b) hp_fun\<close> where
-  \<open>hp_update_nxt i nxt = (\<lambda>(prevs, nxts, childs, scores). (prevs, nxts(i:=nxt), childs, scores))\<close>
+  \<open>hp_update_nxt i nxt = (\<lambda>(prevs, nxts, childs, parents, score). (prevs, nxts(i:=nxt), childs, parents, score))\<close>
+
+definition hp_update_parents :: \<open>'a \<Rightarrow> 'a option \<Rightarrow> ('a, 'b) hp_fun \<Rightarrow> ('a, 'b) hp_fun\<close> where
+  \<open>hp_update_parents i nxt = (\<lambda>(prevs, nxts, childs, parents, score). (prevs, nxts, childs, parents(i:=nxt), score))\<close>
 
 definition hp_update_score :: \<open>'a \<Rightarrow> 'b option \<Rightarrow> ('a, 'b) hp_fun \<Rightarrow> ('a, 'b) hp_fun\<close> where
-  \<open>hp_update_score i nxt = (\<lambda>(prevs, nxts, childs, scores). (prevs, nxts, childs, scores(i:=nxt)))\<close>
+  \<open>hp_update_score i nxt = (\<lambda>(prevs, nxts, childs, parents, score). (prevs, nxts, childs, parents, score(i:=nxt)))\<close>
 
+fun hp_read_nxt :: \<open>_ \<Rightarrow> ('a, 'b) hp_fun \<Rightarrow> _\<close> where \<open>hp_read_nxt i (prevs, nxts, childs) = nxts i\<close>
+fun hp_read_prev :: \<open>_ \<Rightarrow> ('a, 'b) hp_fun \<Rightarrow> _\<close> where \<open>hp_read_prev i (prevs, nxts, childs) = prevs i\<close>
+fun hp_read_child :: \<open>_ \<Rightarrow> ('a, 'b) hp_fun \<Rightarrow> _\<close> where \<open>hp_read_child i (prevs, nxts, childs, parents, scores) = childs i\<close>
+fun hp_read_parent :: \<open>_ \<Rightarrow> ('a, 'b) hp_fun \<Rightarrow> _\<close> where \<open>hp_read_parent i (prevs, nxts, childs, parents, scores) = parents i\<close>
+fun hp_read_score :: \<open>_ \<Rightarrow> ('a, 'b) hp_fun \<Rightarrow> _\<close> where \<open>hp_read_score i (prevs, nxts, childs, parents, scores) = scores i\<close>
 
-fun hp_read_nxt :: \<open>_ \<Rightarrow> ('a, 'b) hp_fun  \<Rightarrow> _\<close> where \<open>hp_read_nxt i (prevs, nxts, childs) = nxts i\<close>
-fun hp_read_prev :: \<open>_ \<Rightarrow> ('a, 'b) hp_fun  \<Rightarrow> _\<close> where \<open>hp_read_prev i (prevs, nxts, childs) = prevs i\<close>
-fun hp_read_child :: \<open>_ \<Rightarrow> ('a, 'b) hp_fun  \<Rightarrow> _\<close> where \<open>hp_read_child i (prevs, nxts, childs, scores) = childs i\<close>
-fun hp_read_score :: \<open>_ \<Rightarrow> ('a, 'b) hp_fun  \<Rightarrow> _\<close> where \<open>hp_read_score i (prevs, nxts, childs, scores) = scores i\<close>
-
-definition encoded_hp_prop :: \<open>('e,'f) hp multiset \<Rightarrow> _\<close> where
-  \<open>encoded_hp_prop m = (\<lambda>(prevs,nxts,children, scores). distinct_mset (\<Sum>\<^sub># (mset_nodes `# m)) \<and>
+definition encoded_hp_prop :: \<open>('e,'f) hp multiset \<Rightarrow>  ('e, 'f) hp_fun \<Rightarrow> _\<close> where
+  \<open>encoded_hp_prop m = (\<lambda>(prevs,nxts,children, parents, scores). distinct_mset (\<Sum>\<^sub># (mset_nodes `# m)) \<and>
      (\<forall>m\<in># m. \<forall>x \<in># mset_nodes m. prevs x = map_option node (hp_prev x m)) \<and>
      (\<forall>m'\<in>#m. \<forall>x \<in># mset_nodes m'. nxts x = map_option node (hp_next x m')) \<and>
      (\<forall>m\<in># m. \<forall>x \<in># mset_nodes m. children x = map_option node (hp_child x m)) \<and>
+     (\<forall>m\<in># m. \<forall>x \<in># mset_nodes m. parents x = map_option node (hp_parent x m)) \<and>
      (\<forall>m\<in># m. \<forall>x \<in># mset_nodes m. scores x = map_option score (hp_node x m)))\<close>
 
 lemma encoded_hp_prop_irrelevant:
   assumes \<open>a \<notin># \<Sum>\<^sub># (mset_nodes `# m)\<close> and
-    \<open>encoded_hp_prop m (nxts, prevs, children, scores)\<close>
+    \<open>encoded_hp_prop m (nxts, prevs, children, parents, scores)\<close>
   shows
-    \<open>encoded_hp_prop (add_mset (Hp a sc []) m) (nxts(a:= None), prevs(a:=None), children(a:=None), scores(a:=Some sc))\<close>
+    \<open>encoded_hp_prop (add_mset (Hp a sc []) m) (nxts(a:= None), prevs(a:=None), children(a:=None), parents(a:=None), scores(a:=Some sc))\<close>
   using assms by (auto simp: encoded_hp_prop_def)
 
+lemma hp_parent_single_child[simp]: \<open>hp_parent (node a) (Hp m w\<^sub>m [a]) = Some (Hp m w\<^sub>m [a])\<close>
+  by (cases a) (auto simp: hp_parent.simps(1))
+
+lemma hp_parent_children_single_hp_parent[simp]: \<open>hp_parent_children b [a] = hp_parent b a\<close>
+  by (auto simp: hp_parent_children_def)
+
+
+lemma hp_parent_single_child_If:
+  \<open>b \<noteq> m \<Longrightarrow> hp_parent b (Hp m w\<^sub>m (a # [])) = (if b = node a then Some (Hp m w\<^sub>m [a]) else hp_parent b a)\<close>
+  by (auto simp: hp_parent_simps)
+
+lemma hp_parent_single_child_If2:
+  \<open>distinct_mset (add_mset m (mset_nodes a)) \<Longrightarrow>
+  hp_parent b (Hp m w\<^sub>m (a # [])) = (if b = m then None else if b = node a then Some (Hp m w\<^sub>m [a]) else hp_parent b a)\<close>
+  by (auto simp: hp_parent_simps)
+
+
+lemma hp_parent_single_child_If3:
+  \<open>distinct_mset (add_mset m (mset_nodes a + sum_list (map mset_nodes xs))) \<Longrightarrow>
+  hp_parent b (Hp m w\<^sub>m (a # xs)) = (if b = m then None else if b = node a then Some (Hp m w\<^sub>m (a # xs)) else hp_parent_children b (a # xs))\<close>
+  by (auto simp: hp_parent_simps)
+
+lemma hp_parent_is_first_child[simp]: \<open>hp_parent (node a) (Hp m w\<^sub>m (a # ch\<^sub>m)) = Some (Hp m w\<^sub>m (a # ch\<^sub>m))\<close>
+  by (auto simp: hp_parent.simps(1))
+
+lemma hp_parent_children_in_first_child[simp]: \<open>distinct_mset (mset_nodes a + sum_list (map mset_nodes ch\<^sub>m)) \<Longrightarrow>
+  xa \<in># mset_nodes a \<Longrightarrow> hp_parent_children xa (a # ch\<^sub>m) = hp_parent xa a\<close>
+  by (auto simp: hp_parent_children_cons split: option.splits dest: multi_member_split)
 
 lemma encoded_hp_prop_link:
-  fixes ch\<^sub>m a prevs
+  fixes ch\<^sub>m a prevs parents m
   defines \<open>prevs' \<equiv> (if ch\<^sub>m = [] then prevs else prevs (node (hd ch\<^sub>m) := Some (node a)))\<close>
-  assumes \<open>encoded_hp_prop (add_mset (Hp m w\<^sub>m ch\<^sub>m) (add_mset a x)) (prevs, nxts, children, scores)\<close>
+  defines \<open>parents' \<equiv> (if ch\<^sub>m = [] then parents else parents (node (hd ch\<^sub>m) := None))\<close>
+  assumes \<open>encoded_hp_prop (add_mset (Hp m w\<^sub>m ch\<^sub>m) (add_mset a x)) (prevs, nxts, children, parents, scores)\<close>
   shows
-    \<open>encoded_hp_prop (add_mset (Hp m w\<^sub>m (a # ch\<^sub>m)) x) (prevs', nxts(node a:= if ch\<^sub>m = [] then None else Some (node (hd ch\<^sub>m))), children(m := Some (node a)), scores(m:=Some w\<^sub>m))\<close>
+    \<open>encoded_hp_prop (add_mset (Hp m w\<^sub>m (a # ch\<^sub>m)) x) (prevs', nxts(node a:= if ch\<^sub>m = [] then None else Some (node (hd ch\<^sub>m))),
+      children(m := Some (node a)), parents'(node a:= Some m), scores(m:=Some w\<^sub>m))\<close>
 proof -
   have H[simp]: \<open>distinct_mset (sum_list (map mset_nodes ch\<^sub>m) + (mset_nodes a))\<close> \<open>distinct_mset (mset_nodes a)\<close>
-    using assms unfolding encoded_hp_prop_def prod.simps
-    by (metis distinct_mset_add mset_nodes_simps sum_mset.insert sum_mset_sum_list union_assoc)+
+     \<open>distinct_mset (sum_list (map mset_nodes ch\<^sub>m))\<close> and
+    dist: \<open>distinct_mset (sum_list (map mset_nodes ch\<^sub>m) + (mset_nodes a) + \<Sum>\<^sub># (mset_nodes `# x))\<close>
+      \<open>m \<notin># sum_list (map mset_nodes ch\<^sub>m) + (mset_nodes a) + \<Sum>\<^sub># (mset_nodes `# x)\<close>
+    using assms unfolding encoded_hp_prop_def prod.simps apply auto
+    by (metis distinct_mset_add mset_nodes_simps sum_mset.insert union_assoc)+
+  have [simp]: \<open>distinct_mset (mset_nodes a + sum_list (map mset_nodes ch\<^sub>m))\<close>
+    by (metis H(1) union_ac(2))
+  have 1: \<open>ch\<^sub>m \<noteq> [] \<Longrightarrow> node a \<noteq> node (hd ch\<^sub>m)\<close>
+    if \<open>distinct_mset (sum_list (map mset_nodes ch\<^sub>m) + (mset_nodes a + \<Sum>\<^sub># (mset_nodes `# x)))\<close>
+    using that by (cases ch\<^sub>m; cases a; auto)
   have K: \<open>xa \<in># mset_nodes a \<Longrightarrow> xa \<notin># sum_list (map mset_nodes ch\<^sub>m)\<close>
-    \<open>xa \<in># sum_list (map mset_nodes ch\<^sub>m) \<Longrightarrow> xa \<notin># mset_nodes a\<close> for xa
+    \<open>xa \<in># sum_list (map mset_nodes ch\<^sub>m) \<Longrightarrow> xa \<notin># mset_nodes a\<close>for xa
     using H by (auto simp del: H dest!: multi_member_split)
+
+  have [simp]: \<open>ch\<^sub>m \<noteq> [] \<Longrightarrow> ma \<in># x \<Longrightarrow> hp_parent (node (hd ch\<^sub>m)) ma = None\<close>
+    \<open>ma \<in># x \<Longrightarrow> hp_parent (node a) ma = None\<close>
+    \<open>ma \<in># x \<Longrightarrow> node a \<notin># mset_nodes ma\<close> for ma
+    by (cases ch\<^sub>m; cases \<open>hd ch\<^sub>m\<close>; cases a; use dist in \<open>auto simp del: H dest!: multi_member_split\<close>; fail)+
+  have [simp]: \<open>xa \<in># sum_list (map mset_nodes ch\<^sub>m) \<Longrightarrow> xa \<noteq> node (hd ch\<^sub>m) \<Longrightarrow> 
+    (hp_parent xa (Hp m w\<^sub>m ch\<^sub>m)) = (hp_parent_children xa (a # ch\<^sub>m))\<close> for xa
+    using dist H
+    by (cases ch\<^sub>m; cases x)
+     (auto simp: hp_parent_single_child_If3 hp_parent_children_cons
+      simp del: H
+      dest!: multi_member_split split: option.splits)
+
   show ?thesis
-    using assms unfolding encoded_hp_prop_def prod.simps
+    using assms 1 unfolding encoded_hp_prop_def prod.simps
     apply (intro conjI impI ballI)
     subgoal by (auto simp: ac_simps)
     subgoal
@@ -77,20 +132,24 @@ proof -
     subgoal
       by (auto split: option.splits simp: K)
     subgoal
+      by (auto simp: hp_parent_single_child_If2 hp_parent_single_child_If3)
+    subgoal
       by (auto split: option.splits simp: K(2))
     done
 qed
 
 
 definition encoded_hp_prop_list :: \<open>('e,'f) hp multiset \<Rightarrow> ('e,'f) hp list \<Rightarrow> _\<close> where
-  \<open>encoded_hp_prop_list m xs  = (\<lambda>(prevs,nxts,children, scores). distinct_mset (\<Sum>\<^sub># (mset_nodes `# m + mset_nodes `# (mset xs))) \<and>
+  \<open>encoded_hp_prop_list m xs  = (\<lambda>(prevs,nxts,children, parents, scores). distinct_mset (\<Sum>\<^sub># (mset_nodes `# m + mset_nodes `# (mset xs))) \<and>
      (\<forall>m'\<in>#m. \<forall>x \<in># mset_nodes m'. nxts x = map_option node (hp_next x m')) \<and>
      (\<forall>m\<in># m. \<forall>x \<in># mset_nodes m. prevs x = map_option node (hp_prev x m)) \<and>
      (\<forall>m\<in># m. \<forall>x \<in># mset_nodes m. children x = map_option node (hp_child x m)) \<and>
+     (\<forall>m\<in># m. \<forall>x \<in># mset_nodes m. parents x = map_option node (hp_parent x m)) \<and>
      (\<forall>m\<in># m. \<forall>x \<in># mset_nodes m. scores x = map_option score (hp_node x m)) \<and>
      (\<forall>x \<in># \<Sum>\<^sub># (mset_nodes `# mset xs). nxts x = map_option node (hp_next_children x xs)) \<and>
      (\<forall>x \<in># \<Sum>\<^sub># (mset_nodes `# mset xs). prevs x = map_option node (hp_prev_children x xs)) \<and>
      (\<forall>x \<in># \<Sum>\<^sub># (mset_nodes `# mset xs). children x = map_option node (hp_child_children x xs)) \<and>
+     (\<forall>x \<in># \<Sum>\<^sub># (mset_nodes `# mset xs). parents x = map_option node (hp_parent_children x xs)) \<and>
      (\<forall>x \<in># \<Sum>\<^sub># (mset_nodes `# mset xs). scores x = map_option score (hp_node_children x xs))
   )\<close>
 
@@ -101,22 +160,55 @@ lemma encoded_hp_prop_list_encoded_hp_prop_single[simp]: \<open>encoded_hp_prop_
   unfolding encoded_hp_prop_list_def encoded_hp_prop_def by auto
 
 lemma encoded_hp_prop_list_remove_min:
-  assumes \<open>encoded_hp_prop_list (add_mset (Hp a b child) xs) [] (prevs, nxts, children, scores)\<close>
-  shows \<open>encoded_hp_prop_list xs child (prevs, nxts, children(a:=None), scores(a:=None))\<close>
-  using assms
-  unfolding encoded_hp_prop_list_def
-  by (auto simp: ac_simps)
+  fixes parents a child children
+  defines \<open>parents' \<equiv> (if children a = None then parents else parents(the (children a) := None))\<close>
+  assumes \<open>encoded_hp_prop_list (add_mset (Hp a b child) xs) [] (prevs, nxts, children, parents, scores)\<close>
+  shows \<open>encoded_hp_prop_list xs child (prevs, nxts, children(a:=None), parents', scores(a:=None))\<close>
+proof -
+  have a: \<open>children a = None \<longleftrightarrow> child = []\<close> and
+    b: \<open>children a \<noteq> None \<Longrightarrow> the (children a) = node (hd child)\<close>
+    using assms
+    unfolding encoded_hp_prop_list_def
+    by (cases child; auto simp: ac_simps hp_parent_single_child_If3 dest: multi_member_split; fail)+
+  show ?thesis
+    using assms b
+    unfolding encoded_hp_prop_list_def a
+    apply (cases child)
+    apply (auto simp: ac_simps hp_parent_single_child_If3 dest: multi_member_split)
+    apply (metis UnCI add_diff_cancel_left' distinct_mset_in_diff image_msetI in_Union_mset_iff node_in_mset_nodes set_mset_union)
+    apply (metis hp_child.simps(1) hp_child_hp_children_simps2)
+    apply (metis hp_node_None_notin2 option.case_eq_if option.exhaust_sel)
+    apply (metis distinct_mset_add hp_parent_children_itself union_ac(1))
+    apply (metis hp_parent_simps(2))
+    by (metis hp_parent_simps(2))
+qed
 
+lemma hp_parent_children_skip_first[simp]:
+  \<open>x \<in># sum_list (map mset_nodes ch') \<Longrightarrow>
+  distinct_mset (sum_list (map mset_nodes ch) + sum_list (map mset_nodes ch')) \<Longrightarrow>
+  hp_parent_children x (ch @ ch') = hp_parent_children x ch'\<close>
+  by (induction ch) (auto simp: hp_parent_children_cons dest!: multi_member_split)
+
+lemma hp_parent_children_skip_last[simp]:
+  \<open>x \<in># sum_list (map mset_nodes ch) \<Longrightarrow>
+  distinct_mset (sum_list (map mset_nodes ch) + sum_list (map mset_nodes ch')) \<Longrightarrow>
+  hp_parent_children x (ch @ ch') = hp_parent_children x ch\<close>
+  by (induction ch) (auto simp: hp_parent_children_cons dest!: multi_member_split split: option.splits)
+
+lemma hp_parent_first_child[simp]:
+  \<open>n \<noteq> m \<Longrightarrow> hp_parent n (Hp m w\<^sub>m (Hp n w\<^sub>n ch\<^sub>n # ch\<^sub>m)) = Some (Hp m w\<^sub>m (Hp n w\<^sub>n ch\<^sub>n # ch\<^sub>m))\<close>
+  by (auto simp: hp_parent.simps(1))
 
 lemma encoded_hp_prop_list_link:
-  fixes m ch\<^sub>m prevs b hp\<^sub>m n nxts children
+  fixes m ch\<^sub>m prevs b hp\<^sub>m n nxts children parents
   defines \<open>prevs\<^sub>0 \<equiv> (if ch\<^sub>m = [] then prevs else prevs (node (hd ch\<^sub>m) := Some n))\<close>
   defines \<open>prevs' \<equiv> (if b = [] then prevs\<^sub>0 else prevs\<^sub>0 (node (hd b) := Some m)) (n:= None)\<close>
   defines \<open>nxts' \<equiv> nxts (m := map_option node (option_hd b), n := map_option node (option_hd ch\<^sub>m))\<close>
   defines \<open>children' \<equiv> children (m := Some n)\<close>
-  assumes \<open>encoded_hp_prop_list (xs) (a @ [Hp m w\<^sub>m ch\<^sub>m, Hp n w\<^sub>n ch\<^sub>n] @ b) (prevs, nxts, children, scores)\<close>
+  defines \<open>parents' \<equiv> (if ch\<^sub>m = [] then parents else parents(node (hd ch\<^sub>m) := None))(n := Some m)\<close>
+  assumes \<open>encoded_hp_prop_list (xs) (a @ [Hp m w\<^sub>m ch\<^sub>m, Hp n w\<^sub>n ch\<^sub>n] @ b) (prevs, nxts, children, parents, scores)\<close>
   shows \<open>encoded_hp_prop_list xs (a @ [Hp m w\<^sub>m (Hp n w\<^sub>n ch\<^sub>n # ch\<^sub>m)] @ b)
-       (prevs', nxts', children', scores)\<close>
+       (prevs', nxts', children', parents', scores)\<close>
 proof -
   have dist: \<open>distinct_mset (sum_list (map mset_nodes ch\<^sub>m) + (sum_list (map mset_nodes ch\<^sub>n) +
     (\<Sum>\<^sub># (mset_nodes `# xs) + (sum_list (map mset_nodes a) + sum_list (map mset_nodes b)))))\<close>
@@ -129,15 +221,18 @@ proof -
     \<open>m \<notin># sum_list (map mset_nodes ch\<^sub>n)\<close>
     \<open>m \<notin># sum_list (map mset_nodes a)\<close>
     \<open>m \<notin># sum_list (map mset_nodes b)\<close>
-    \<open>n \<noteq> m\<close> and
+    \<open>n \<noteq> m\<close> \<open>m \<noteq> n\<close> and
     nxts1: \<open>(\<forall>m'\<in>#xs. \<forall>x\<in>#mset_nodes m'. nxts x = map_option node (hp_next x m'))\<close> and
     prevs1: ‹(\<forall>m\<in>#xs. \<forall>x\<in>#mset_nodes m. prevs x = map_option node (hp_prev x m))\<close> and
+    parents1: ‹(\<forall>m\<in>#xs. \<forall>x\<in>#mset_nodes m. parents x = map_option node (hp_parent x m))\<close> and
     child1: \<open>(\<forall>m\<in>#xs. \<forall>x\<in>#mset_nodes m. children x = map_option node (hp_child x m))\<close> and
     scores1: \<open>(\<forall>m\<in>#xs. \<forall>x\<in>#mset_nodes m. scores x = map_option score (hp_node x m))\<close> and
     nxts2: \<open>(\<forall>x\<in>#\<Sum>\<^sub># (mset_nodes `# mset (a @ [Hp m w\<^sub>m ch\<^sub>m, Hp n w\<^sub>n ch\<^sub>n] @ b)).
      nxts x = map_option node (hp_next_children x (a @ [Hp m w\<^sub>m ch\<^sub>m, Hp n w\<^sub>n ch\<^sub>n] @ b)))\<close> and
     prevs2: \<open>(\<forall>x\<in>#\<Sum>\<^sub># (mset_nodes `# mset (a @ [Hp m w\<^sub>m ch\<^sub>m, Hp n w\<^sub>n ch\<^sub>n] @ b)).
      prevs x = map_option node (hp_prev_children x (a @ [Hp m w\<^sub>m ch\<^sub>m, Hp n w\<^sub>n ch\<^sub>n] @ b)))\<close> and
+    parents2: \<open>(\<forall>x\<in>#\<Sum>\<^sub># (mset_nodes `# mset (a @ [Hp m w\<^sub>m ch\<^sub>m, Hp n w\<^sub>n ch\<^sub>n] @ b)).
+     parents x = map_option node (hp_parent_children x (a @ [Hp m w\<^sub>m ch\<^sub>m, Hp n w\<^sub>n ch\<^sub>n] @ b)))\<close> and
     child2: \<open>(\<forall>x\<in>#\<Sum>\<^sub># (mset_nodes `# mset (a @ [Hp m w\<^sub>m ch\<^sub>m, Hp n w\<^sub>n ch\<^sub>n] @ b)).
     children x = map_option node (hp_child_children x (a @ [Hp m w\<^sub>m ch\<^sub>m, Hp n w\<^sub>n ch\<^sub>n] @ b)))\<close> and
     scores2: \<open>(\<forall>x\<in>#\<Sum>\<^sub># (mset_nodes `# mset (a @ [Hp m w\<^sub>m ch\<^sub>m, Hp n w\<^sub>n ch\<^sub>n] @ b)).
@@ -186,7 +281,11 @@ proof -
     using dist that notin by (cases ch\<^sub>m; auto dest: multi_member_split; fail)+
   have [simp]: \<open>m \<noteq> node (hd b)\<close> \<open>n \<noteq> node (hd b)\<close> if \<open>b \<noteq> []›
     using dist that notin unfolding encoded_hp_prop_list_def by (cases b; auto; fail)+
-
+  have [simp]: \<open>ma \<in># xs \<Longrightarrow> node (hd ch\<^sub>m) \<notin># mset_nodes ma\<close> if \<open>ch\<^sub>m \<noteq> []› for ma
+    using dist that notin by (cases ch\<^sub>m; auto dest!: multi_member_split; fail)+
+  have [simp]: \<open>hp_parent_children (node (hd ch\<^sub>m)) ch\<^sub>m = None\<close>
+    by (metis \<open>distinct_mset (sum_list (map mset_nodes a) + sum_list (map mset_nodes ch\<^sub>m))\<close> distinct_mset_add
+      hp_parent.simps(2) hp_parent_None_iff_children_None hp_parent_children_hd_None sum_image_mset_sum_map)
   define NOTIN where
     \<open>NOTIN x ch\<^sub>n \<equiv> x \<notin># sum_list (map mset_nodes ch\<^sub>n)\<close> for x and  ch\<^sub>n :: \<open>('a, 'b) hp list\<close>
   have K[unfolded NOTIN_def[symmetric]]: \<open>x \<in># sum_list (map mset_nodes ch\<^sub>n) \<Longrightarrow> x \<notin># sum_list (map mset_nodes a)\<close>
@@ -215,7 +314,7 @@ proof -
     using dist notin by (auto dest!: multi_member_split simp: NOTIN_def)
   note [simp] = NOTIN_def[symmetric]
   show ?thesis
-    using dist2 unfolding encoded_hp_prop_list_def prod.simps assms(1,2,3,4)
+    using dist2 unfolding encoded_hp_prop_list_def prod.simps assms(1-5)
     apply (intro conjI impI allI)
     subgoal using assms unfolding encoded_hp_prop_list_def
       by (auto simp: ac_simps simp del: NOTIN_def[symmetric])
@@ -229,6 +328,9 @@ proof -
       done
     subgoal
       using child1
+      by auto
+    subgoal
+      using parents1
       by auto
     subgoal
       using scores1
@@ -249,6 +351,15 @@ proof -
         hp_child_children_skip_first[of _ _ \<open>[_]\<close>, simplified]
         split: option.splits)
     subgoal
+      using parents2 notin(9)
+      by (auto simp add: K K' K'' hp_parent_children_skip_first[of _ \<open>[_]\<close>, simplified]
+        hp_parent_children_skip_first[of _ \<open>_ # _\<close>, simplified] hp_parent_simps_single_if
+        hp_parent_children_skip_last[of _ _ \<open>[_]\<close>, simplified]
+        hp_parent_children_skip_last[of _ \<open>[_]\<close>, simplified] notin
+        hp_parent_children_skip_last[of _ \<open>[_, _]\<close>, simplified]
+        hp_parent_children_skip_first[of _ _ \<open>[_]\<close>, simplified]
+        split: option.splits)
+    subgoal
       using scores2
       by (auto split: option.splits simp: K K' K'' hp_node_children_Cons_if
         ex_hp_node_children_Some_in_mset_nodes
@@ -257,14 +368,15 @@ proof -
 qed
 
 lemma encoded_hp_prop_list_link2:
-  fixes m ch\<^sub>m prevs b hp\<^sub>m n nxts children ch\<^sub>n a
+  fixes m ch\<^sub>m prevs b hp\<^sub>m n nxts children ch\<^sub>n a parents
   defines \<open>prevs' \<equiv> (if ch\<^sub>n = [] then prevs else prevs (node (hd ch\<^sub>n) := Some m))(m := None, n := map_option node (option_last a))\<close>
   defines \<open>nxts\<^sub>0 \<equiv> (if a = [] then nxts else nxts(node (last a) := Some n))\<close>
   defines \<open>nxts' \<equiv> nxts\<^sub>0 (n := map_option node (option_hd b), m := map_option node (option_hd ch\<^sub>n))\<close>
   defines \<open>children' \<equiv> children (n := Some m)\<close>
-  assumes \<open>encoded_hp_prop_list (xs) (a @ [Hp m w\<^sub>m ch\<^sub>m, Hp n w\<^sub>n ch\<^sub>n] @ b) (prevs, nxts, children, scores)\<close>
+  defines \<open>parents' \<equiv> (if ch\<^sub>n = [] then parents else parents(node (hd ch\<^sub>n) := None))(m := Some n)\<close>
+  assumes \<open>encoded_hp_prop_list (xs) (a @ [Hp m w\<^sub>m ch\<^sub>m, Hp n w\<^sub>n ch\<^sub>n] @ b) (prevs, nxts, children, parents, scores)\<close>
   shows \<open>encoded_hp_prop_list xs (a @ [Hp n w\<^sub>n (Hp m w\<^sub>m ch\<^sub>m # ch\<^sub>n)] @ b)
-       (prevs', nxts', children', scores)\<close>
+       (prevs', nxts', children', parents', scores)\<close>
 proof -
   have dist: \<open>distinct_mset (sum_list (map mset_nodes ch\<^sub>m) + (sum_list (map mset_nodes ch\<^sub>n) +
     (\<Sum>\<^sub># (mset_nodes `# xs) + (sum_list (map mset_nodes a) + sum_list (map mset_nodes b)))))\<close>
@@ -281,12 +393,15 @@ proof -
     nxts1: \<open>(\<forall>m'\<in>#xs. \<forall>x\<in>#mset_nodes m'. nxts x = map_option node (hp_next x m'))\<close> and
     prevs1: ‹(\<forall>m\<in>#xs. \<forall>x\<in>#mset_nodes m. prevs x = map_option node (hp_prev x m))\<close> and
     child1: \<open>(\<forall>m\<in>#xs. \<forall>x\<in>#mset_nodes m. children x = map_option node (hp_child x m))\<close> and
+    parent1: ‹(\<forall>m\<in>#xs. \<forall>x\<in>#mset_nodes m. parents x = map_option node (hp_parent x m))\<close> and
     nxts2: \<open>(\<forall>x\<in>#\<Sum>\<^sub># (mset_nodes `# mset (a @ [Hp m w\<^sub>m ch\<^sub>m, Hp n w\<^sub>n ch\<^sub>n] @ b)).
      nxts x = map_option node (hp_next_children x (a @ [Hp m w\<^sub>m ch\<^sub>m, Hp n w\<^sub>n ch\<^sub>n] @ b)))\<close> and
     prevs2: \<open>(\<forall>x\<in>#\<Sum>\<^sub># (mset_nodes `# mset (a @ [Hp m w\<^sub>m ch\<^sub>m, Hp n w\<^sub>n ch\<^sub>n] @ b)).
      prevs x = map_option node (hp_prev_children x (a @ [Hp m w\<^sub>m ch\<^sub>m, Hp n w\<^sub>n ch\<^sub>n] @ b)))\<close> and
     child2: \<open>(\<forall>x\<in>#\<Sum>\<^sub># (mset_nodes `# mset (a @ [Hp m w\<^sub>m ch\<^sub>m, Hp n w\<^sub>n ch\<^sub>n] @ b)).
     children x = map_option node (hp_child_children x (a @ [Hp m w\<^sub>m ch\<^sub>m, Hp n w\<^sub>n ch\<^sub>n] @ b)))\<close> and
+    parent2: \<open>(\<forall>x\<in>#\<Sum>\<^sub># (mset_nodes `# mset (a @ [Hp m w\<^sub>m ch\<^sub>m, Hp n w\<^sub>n ch\<^sub>n] @ b)).
+     parents x = map_option node (hp_parent_children x (a @ [Hp m w\<^sub>m ch\<^sub>m, Hp n w\<^sub>n ch\<^sub>n] @ b)))\<close> and
     scores2: \<open>(\<forall>x\<in>#\<Sum>\<^sub># (mset_nodes `# mset (a @ [Hp m w\<^sub>m ch\<^sub>m, Hp n w\<^sub>n ch\<^sub>n] @ b)).
       scores x = map_option score (hp_node_children x (a @ [Hp m w\<^sub>m ch\<^sub>m, Hp n w\<^sub>n ch\<^sub>n] @ b)))\<close> and
     scores1: \<open>(\<forall>m\<in>#xs. \<forall>x\<in>#mset_nodes m. scores x = map_option score (hp_node x m))\<close> and
@@ -344,6 +459,9 @@ proof -
   have [simp]: \<open>m \<noteq> node (hd ch\<^sub>m)\<close> \<open>n \<noteq> node (hd ch\<^sub>m)\<close> \<open>(node (hd ch\<^sub>m)) \<notin># sum_list (map mset_nodes b)\<close>
     \<open>node (hd ch\<^sub>m) \<notin># sum_list (map mset_nodes ch\<^sub>n)\<close>if \<open>ch\<^sub>m \<noteq> []›
     using dist that notin by (cases ch\<^sub>m; auto dest: multi_member_split; fail)+
+  have [simp]: \<open>m \<noteq> node (hd ch\<^sub>n)\<close> \<open>n \<noteq> node (hd ch\<^sub>n)\<close> \<open>(node (hd ch\<^sub>n)) \<notin># sum_list (map mset_nodes b)\<close>
+    \<open>node (hd ch\<^sub>n) \<notin># sum_list (map mset_nodes ch\<^sub>m)\<close>if \<open>ch\<^sub>n \<noteq> []›
+    using dist that notin by (cases ch\<^sub>n; auto dest: multi_member_split; fail)+
   have [simp]: \<open>m \<noteq> node (hd b)\<close> \<open>n \<noteq> node (hd b)\<close> if \<open>b \<noteq> []›
     using dist that notin unfolding encoded_hp_prop_list_def by (cases b; auto; fail)+
 
@@ -377,11 +495,18 @@ proof -
     \<open>node (last a) \<notin># sum_list (map mset_nodes ch\<^sub>n)\<close> if \<open>a \<noteq> []\<close>
     using that dist by (cases a rule: rev_cases; cases \<open>last a\<close>; auto; fail)+
   note [simp] = NOTIN_def[symmetric]
-  have [iff]: \<open> ch\<^sub>n \<noteq> [] \<Longrightarrow> ma \<in># xs \<Longrightarrow> node (hd ch\<^sub>n) \<in># mset_nodes ma \<longleftrightarrow> False\<close> for ma
+
+  have [simp]: \<open>hp_parent_children (node (hd ch\<^sub>m)) ch\<^sub>m = None\<close>
+    by (metis \<open>distinct_mset (sum_list (map mset_nodes a) + sum_list (map mset_nodes ch\<^sub>m))\<close> distinct_mset_add
+      hp_parent.simps(2) hp_parent_None_iff_children_None hp_parent_children_hd_None sum_image_mset_sum_map)
+  have [simp]: \<open>ch\<^sub>n \<noteq> [] \<Longrightarrow> hp_parent_children (node (hd ch\<^sub>n)) ch\<^sub>n = None\<close>
+    using dist
+    by (cases ch\<^sub>n; cases \<open>hd ch\<^sub>n\<close>) (auto simp: hp_parent_children_cons distinct_mset_add split: option.splits)
+  have [iff]: \<open>ch\<^sub>n \<noteq> [] \<Longrightarrow> ma \<in># xs \<Longrightarrow> node (hd ch\<^sub>n) \<in># mset_nodes ma \<longleftrightarrow> False\<close> for ma
     using dist2 apply auto
     by (metis (no_types, lifting) add_mset_disjoint(1) distinct_mset_add insert_DiffM inter_mset_empty_distrib_right node_hd_in_sum sum_mset.insert)
   show ?thesis
-    using dist2 unfolding encoded_hp_prop_list_def prod.simps assms(1,2,3,4)
+    using dist2 unfolding encoded_hp_prop_list_def prod.simps assms(1-5)
     apply (intro conjI impI allI)
     subgoal using assms unfolding encoded_hp_prop_list_def
       by (auto simp: ac_simps simp del: NOTIN_def[symmetric])
@@ -393,6 +518,9 @@ proof -
       by auto
     subgoal
       using child1
+      by auto
+    subgoal
+      using parent1
       by auto
     subgoal
       using scores1
@@ -414,6 +542,17 @@ proof -
         hp_child_children_skip_last[of _ \<open>[_, _]\<close>, simplified]
         hp_child_children_skip_first[of _ _ \<open>[_,_]\<close>, simplified]
         hp_child_children_skip_first[of _ _ \<open>[_]\<close>, simplified]
+        split: option.splits)
+    subgoal
+      using parent2 notin(9)
+      by (auto simp add: K K' K'' hp_parent_children_skip_first[of _ \<open>[_]\<close>, simplified]
+        hp_parent_children_skip_first[of _ \<open>_ # _\<close>, simplified] hp_parent_simps_single_if
+        hp_parent_children_skip_last[of _ _ \<open>[_]\<close>, simplified]
+        hp_parent_children_skip_last[of _ \<open>[_]\<close>, simplified] notin
+        hp_parent_children_skip_last[of _ \<open>[_, _]\<close>, simplified]
+        hp_parent_children_skip_first[of _ _ \<open>[_]\<close>, simplified]
+        hp_parent_children_skip_first[of _ _ \<open>[_,_]\<close>, simplified]
+        eq_commute[of n \<open>node (hd [])\<close>]
         split: option.splits)
     subgoal
       using scores2
@@ -446,8 +585,8 @@ lemma encoded_hp_prop_list_update_score:
   shows \<open>encoded_hp_prop_list (add_mset (Hp a x c) hs) []
         arr'\<close>
 proof -
-  obtain prevs nxts childs scores \<V> where
-    arr: \<open>arr = ((prevs, nxts, childs, scores))\<close> and
+  obtain prevs nxts childs parents scores \<V> where
+    arr: \<open>arr = ((prevs, nxts, childs, parents, scores))\<close> and
     dist: \<open>distinct_mset (sum_list (map mset_nodes c) + \<Sum>\<^sub># (mset_nodes `# hs))\<close>
       \<open>a \<notin># sum_list (map mset_nodes c)\<close>
       \<open>a \<notin># \<Sum>\<^sub># (mset_nodes `# hs)\<close>
@@ -455,18 +594,20 @@ proof -
     \<V>: \<open>set_mset (sum_list (map mset_nodes xs)) \<subseteq> \<V>\<close>
     by (cases arr) (use assms in \<open>auto simp: ac_simps encoded_hp_prop_list2_conc_def encoded_hp_prop_list_def
         encoded_hp_prop_def\<close>)
-  have find_key_in_nodes: \<open>VSIDS.find_key a h \<noteq> None \<Longrightarrow> node (the (VSIDS.find_key a h)) \<in># mset_nodes h\<close>
+  have find_key_in_nodes: \<open>find_key a h \<noteq> None \<Longrightarrow> node (the (find_key a h)) \<in># mset_nodes h\<close>
     by (cases \<open>a \<in># mset_nodes h\<close>)
    	 (use find_key_None_or_itself[of a h] in \<open>auto simp del: find_key_None_or_itself\<close>)
-  have in_find_key_in_nodes1: \<open>x \<in># mset_nodes y \<Longrightarrow> VSIDS.find_key a h = Some y \<Longrightarrow> x \<in># mset_nodes h\<close> for x y
+  have in_find_key_in_nodes1: \<open>x \<in># mset_nodes y \<Longrightarrow> find_key a h = Some y \<Longrightarrow> x \<in># mset_nodes h\<close> for x y
     using mset_nodes_find_key_subset[of a h]
     by auto
-  have [simp]: \<open>VSIDS.find_key a h = None \<Longrightarrow> VSIDS.remove_key a h = Some h\<close>
-    by (metis VSIDS.find_key.simps find_key_none_iff hp.exhaust_sel hp_node_None_notin2
+  have [simp]: \<open>find_key a h = None \<Longrightarrow> remove_key a h = Some h\<close>
+    by (metis find_key.simps find_key_none_iff hp.exhaust_sel hp_node_None_notin2
       hp_node_children_None_notin2 hp_node_children_simps2 option_last_Nil option_last_Some_iff(2)
       remove_key_notin_unchanged)
-  have \<open>VSIDS.remove_key a h \<noteq> None \<Longrightarrow> node (the (VSIDS.remove_key a h)) \<in># mset_nodes h\<close>
-    by (metis VSIDS.remove_key.simps get_min2.simps hp.exhaust_sel option.collapse option.distinct(2) remove_key_notin_unchanged)
+  have [simp]: \<open>map_option node (hp_parent xa (Hp a b c)) = map_option node (hp_parent xa (Hp a x c))\<close> for xa
+    by (cases c; auto simp: hp_parent.simps(1))
+  have \<open>remove_key a h \<noteq> None \<Longrightarrow> node (the (remove_key a h)) \<in># mset_nodes h\<close>
+    by (metis remove_key.simps get_min2.simps hp.exhaust_sel option.collapse option.distinct(2) remove_key_notin_unchanged)
   then show ?thesis
     supply [[goals_limit=1]]
     using enc
@@ -492,6 +633,10 @@ proof -
       by (auto simp: find_remove_mset_nodes_full hp_update_score_def)
     subgoal
       by (auto simp: find_remove_mset_nodes_full hp_update_score_def)
+    subgoal
+      by (auto simp: find_remove_mset_nodes_full hp_update_score_def)
+    subgoal
+      by (auto simp: find_remove_mset_nodes_full hp_update_score_def)
     done
 qed
 
@@ -502,7 +647,7 @@ definition hp_insert :: \<open>'a \<Rightarrow> 'b::linorder \<Rightarrow> 'a se
   \<open>hp_insert = (\<lambda>(i::'a) (w::'b) (\<V>::'a set, arr :: ('a, 'b) hp_fun, h :: 'a option). do {
   if h = None then do {
     ASSERT (i \<in> \<V>);
-    RETURN (\<V>, hp_set_all i None None None (Some w) arr, Some i)
+    RETURN (\<V>, hp_set_all i None None None None (Some w) arr, Some i)
    } else do {
     ASSERT (i \<in> \<V>);
     let (j::'a) = ((the h) :: 'a);
@@ -512,14 +657,17 @@ definition hp_insert :: \<open>'a \<Rightarrow> 'b::linorder \<Rightarrow> 'a se
     let y = (the (hp_read_score j arr)::'b);
     if y < w
     then do {
-      let arr = hp_set_all i None None (Some j) (Some (w::'b)) (arr::('a, 'b) hp_fun);
+      let arr = hp_set_all i None None (Some j) None (Some (w::'b)) (arr::('a, 'b) hp_fun);
+      let arr = hp_update_parents j (Some i) arr;
+      let nxt = hp_read_nxt j arr;
       RETURN (\<V>, arr :: ('a, 'b) hp_fun, Some i)
     }
     else do {
       let child = hp_read_child j arr;
-      let arr = hp_set_all j None None (Some i) (Some y) arr;
-      let arr = hp_set_all i None child None (Some (w::'b)) arr;
+      let arr = hp_set_all j None None (Some i) None (Some y) arr;
+      let arr = hp_set_all i None child None (Some j) (Some (w::'b)) arr;
       let arr = (if child = None then arr else hp_update_prev (the child) (Some i) arr);
+      let arr = (if child = None then arr else hp_update_parents (the child) None arr);
       RETURN (\<V>, arr :: ('a, 'b) hp_fun, h)
     }
    }
@@ -532,38 +680,43 @@ lemma hp_insert_spec:
     \<open>i \<in> fst arr\<close>
   shows \<open>hp_insert i w arr \<le> SPEC (\<lambda>arr. encoded_hp_prop_list_conc arr (VSIDS.insert i w h))\<close>
 proof -
-  obtain prevs nxts childs scores \<V> where
-    arr: \<open>arr = (\<V>, (prevs, nxts, childs, scores), map_option node h)\<close>
+  obtain prevs nxts childs scores parents \<V> where
+    arr: \<open>arr = (\<V>, (prevs, nxts, childs, parents, scores), map_option node h)\<close>
     by (cases arr; cases h) (use assms in \<open>auto simp: encoded_hp_prop_list_conc_def encoded_hp_prop_list_def
         encoded_hp_prop_def\<close>)
 
   have enc: \<open>encoded_hp_prop {#Hp i w [the h]#}
-    (prevs(i := None), nxts(i := None, node (the h) := None), childs(i \<mapsto> node (the h)), scores(i \<mapsto> w))\<close> and
+    (prevs(i := None), nxts(i := None, node (the h) := None), childs(i \<mapsto> node (the h)), parents(i:=None)(node (the h) \<mapsto> i), scores(i \<mapsto> w))\<close> and
     enc2: \<open>encoded_hp_prop {#Hp (node (the h)) (score (the h)) (Hp i w [] # hps (the h))#}
    (if hps (the h) = [] then prevs(i := None) else prevs(i := None)(node (hd (hps (the h))) \<mapsto> node (Hp i w [])),
     nxts  (i := None,  node (Hp i w []) := if hps (the h) = [] then None else Some (node (hd (hps (the h))))),
-    childs(i := None)(node (the h) \<mapsto> node (Hp i w [])), scores(i \<mapsto> w, node (the h) \<mapsto> score (the h)))\<close> (is ?G)if \<open>h \<noteq> None\<close>
+    childs(i := None)(node (the h) \<mapsto> node (Hp i w [])),
+    (if hps (the h) = [] then parents(i := None) else parents(i := None, node (hd (hps (the h))) := None))(node (Hp i w []) \<mapsto> node (the h)),
+    scores(i \<mapsto> w, node (the h) \<mapsto> score (the h)))\<close> (is ?G)
+    if \<open>h \<noteq> None\<close>
   proof -
-    have \<open>encoded_hp_prop {#the h#} (prevs, nxts, childs, scores)\<close>
+    have \<open>encoded_hp_prop {#the h#} (prevs, nxts, childs, parents, scores)\<close>
       using that assms by (auto simp: encoded_hp_prop_list_conc_def encoded_hp_prop_list_def
         encoded_hp_prop_def arr)
     then have 0: \<open>encoded_hp_prop {#Hp i w [], the h#}
-      (prevs(i := None), nxts(i := None), childs(i := None), scores(i \<mapsto> w))\<close>
-      using encoded_hp_prop_irrelevant[of i \<open>{#the h#}\<close> prevs nxts childs scores w] that assms
+      (prevs(i := None), nxts(i := None), childs(i := None), parents(i := None), scores(i \<mapsto> w))\<close>
+      using encoded_hp_prop_irrelevant[of i \<open>{#the h#}\<close> prevs nxts childs parents scores w] that assms
       by auto
     from encoded_hp_prop_link[OF this]
     show \<open>encoded_hp_prop {#Hp i w [the h]#}
-      (prevs(i := None), nxts(i := None, node (the h) := None), childs(i \<mapsto> node (the h)), scores(i \<mapsto> w))\<close>
+      (prevs(i := None), nxts(i := None, node (the h) := None), childs(i \<mapsto> node (the h)), parents(i:=None)(node (the h) \<mapsto> i), scores(i \<mapsto> w))\<close>
       by auto
     from 0 have \<open>encoded_hp_prop {#Hp (node (the h)) (score (the h)) (hps (the h)), Hp i w []#}
-      (prevs(i := None), nxts(i := None), childs(i := None), scores(i \<mapsto> w))\<close>
+      (prevs(i := None), nxts(i := None), childs(i := None), parents(i:=None), scores(i \<mapsto> w))\<close>
       by (cases \<open>the h\<close>) (auto simp: add_mset_commute)
     from encoded_hp_prop_link[OF this]
     show ?G .
   qed
-
-  have [simp]: \<open>encoded_hp_prop {#Hp x1a x2 x3#} (prevs, nxts, childs, scores) \<Longrightarrow> scores x1a = Some x2\<close>
-    \<open>encoded_hp_prop {#Hp x1a x2 x3#} (prevs, nxts, childs, scores) \<Longrightarrow> childs x1a = map_option node (option_hd x3)\<close> for x1a x2 x3
+  have 1: \<open>h \<noteq> None \<Longrightarrow> hps (the h) \<noteq> [] \<Longrightarrow> i \<noteq> node (hd (hps (the h)))\<close>
+    using assms by (cases \<open>the h\<close>; cases \<open>hps (the h)\<close>; cases h) auto
+  have [simp]: \<open>encoded_hp_prop {#Hp x1a x2 x3#} (prevs, nxts, childs, parents, scores) \<Longrightarrow> scores x1a = Some x2\<close>
+    \<open>encoded_hp_prop {#Hp x1a x2 x3#} (prevs, nxts, childs, parents, scores) \<Longrightarrow> parents x1a = None\<close>
+    \<open>encoded_hp_prop {#Hp x1a x2 x3#} (prevs, nxts, childs, parents, scores) \<Longrightarrow> childs x1a = map_option node (option_hd x3)\<close> for x1a x2 x3
     by (auto simp: encoded_hp_prop_def)
   show ?thesis
     using assms
@@ -594,12 +747,12 @@ proof -
     subgoal
       using enc
       by (cases h, simp; cases \<open>the h\<close>)
-        (auto simp: hp_set_all_def encoded_hp_prop_list_conc_def fun_upd_idem)
+        (auto simp: hp_set_all_def encoded_hp_prop_list_conc_def fun_upd_idem hp_update_parents_def)
     subgoal
-      using enc2
+      using enc2 1
       by (cases h, simp; cases \<open>the h\<close>)
-       (auto simp: hp_set_all_def encoded_hp_prop_list_conc_def fun_upd_idem hp_update_prev_def
-        fun_upd_twist)
+        (auto simp: hp_set_all_def encoded_hp_prop_list_conc_def fun_upd_idem hp_update_prev_def
+          fun_upd_twist hp_update_parents_def)
      done
 qed
 
@@ -624,11 +777,12 @@ definition hp_link :: \<open>'a \<Rightarrow> 'a \<Rightarrow> 'a set \<times> (
       @ (if prev \<noteq> None then [the prev] else [])
       @ (if nxt \<noteq> None then [the nxt] else []))
       );
-    let arr = hp_set_all parent prev nxt (Some ch) (Some (w\<^sub>p::'b)) (arr::('a, 'b) hp_fun);
-    let arr = hp_set_all ch None child child\<^sub>c\<^sub>h (Some (w\<^sub>c\<^sub>h::'b)) (arr::('a, 'b) hp_fun);
+    let arr = hp_set_all parent prev nxt (Some ch) None (Some (w\<^sub>p::'b)) (arr::('a, 'b) hp_fun);
+    let arr = hp_set_all ch None child child\<^sub>c\<^sub>h (Some parent) (Some (w\<^sub>c\<^sub>h::'b)) (arr::('a, 'b) hp_fun);
     let arr = (if child = None then arr else hp_update_prev (the child) (Some ch) arr);
     let arr = (if nxt = None then arr else hp_update_prev (the nxt) (Some parent) arr);
     let arr = (if prev = None then arr else hp_update_nxt (the prev) (Some parent) arr);
+    let arr = (if child = None then arr else hp_update_parents (the child) None arr);
     RETURN ((\<V>, arr :: ('a, 'b) hp_fun, h), parent)
  })\<close>
 
@@ -643,8 +797,8 @@ lemma hp_link:
   shows \<open>hp_link i j arr \<le> SPEC (\<lambda>(arr, n). encoded_hp_prop_list2_conc arr (xs @ VSIDS.link x y # ys) \<and>
     n = node (VSIDS.link x y))\<close>
 proof -
-  obtain prevs nxts childs scores \<V> where
-    arr: \<open>arr = (\<V>, (prevs, nxts, childs, scores), None)\<close> and
+  obtain prevs nxts childs parents scores \<V> where
+    arr: \<open>arr = (\<V>, (prevs, nxts, childs, parents, scores), None)\<close> and
     dist: \<open>distinct_mset (\<Sum>\<^sub># (mset_nodes `# (mset (xs @ x # y # ys))))\<close> and
     \<V>: \<open>set_mset (sum_list (map mset_nodes (xs @ x # y # ys))) \<subseteq> \<V>\<close>
     by (cases arr) (use assms in \<open>auto simp: ac_simps encoded_hp_prop_list2_conc_def encoded_hp_prop_list_def
@@ -674,6 +828,8 @@ proof -
     \<open>childs j = map_option node (option_hd ch\<^sub>y)\<close>
     \<open>xs \<noteq> [] \<Longrightarrow> nxts (node (last xs)) = Some i\<close>
     \<open>ys \<noteq> [] \<Longrightarrow> prevs (node (hd ys)) = Some j\<close>
+    \<open>parents i = None\<close>
+    \<open>parents j = None\<close>
     using assms(1) x y apply (auto simp: ac_simps encoded_hp_prop_list2_conc_def encoded_hp_prop_list_def
         encoded_hp_prop_def arr hp_child_children_Cons_if)
     apply (smt (verit) assms(3) hp_next_None_notin_children hp_next_children.elims list.discI list.inject list.sel(1) option_hd_Nil option_hd_Some_hd)
@@ -684,9 +840,29 @@ proof -
       sum_image_mset_sum_map)
     using assms(1) x y apply (cases ys;auto simp: ac_simps encoded_hp_prop_list2_conc_def encoded_hp_prop_list_def
       encoded_hp_prop_def arr)
-      apply (cases \<open>hd ys\<close>)
-      apply (auto simp:)
-      done
+    apply (cases \<open>hd ys\<close>)
+    apply (auto simp:)
+    by (simp add: hp_parent_None_notin_same_hd hp_parent_children_cons)
+
+  have par: \<open>parents j = None› \<open>parents i = None›
+    \<open>ch\<^sub>x \<noteq> [] \<Longrightarrow> parents (node (hd ch\<^sub>x)) = Some i\<close>
+    \<open>ch\<^sub>y \<noteq> [] \<Longrightarrow> parents (node (hd ch\<^sub>y)) = Some j\<close>
+    using assms(1) x y apply (auto simp: ac_simps encoded_hp_prop_list2_conc_def encoded_hp_prop_list_def
+      encoded_hp_prop_def arr hp_child_children_Cons_if)
+    apply (metis hp_parent_None_iff_children_None hp_parent_None_notin_same_hd hp_parent_children_cons hp_parent_hd_None sum_image_mset_sum_map)
+    apply (metis assms(2) hp_parent_children_cons hp_parent_simps_single_if option.simps(5))
+    apply (cases ch\<^sub>y)
+    apply (simp_all add: hp_parent_children_skip_first[of _ _ \<open>[_]\<close>, simplified] distinct_mset_add)
+    apply (subst hp_parent_children_skip_first[of _ _ \<open>[_]\<close>, simplified])
+    apply simp
+    apply simp
+    apply (metis distinct_mset_add inter_mset_empty_distrib_right)
+    apply (subst hp_parent_children_skip_last[of _ \<open>[_]\<close>, simplified])
+    apply simp
+    apply simp
+    apply (metis distinct_mset_add inter_mset_empty_distrib_right)
+    apply simp
+    done
 
   have diff:
     \<open>nxts j \<noteq> Some j\<close>  \<open>nxts j \<noteq> Some i\<close>  \<open>nxts i \<noteq> Some i\<close>
@@ -710,15 +886,16 @@ proof -
        (auto split: if_splits)
   have if_pair: \<open>(if a then (b, c) else (d,f)) = (if a then b else d, if a then c else f)\<close> for a b c d f
     by auto
-  have enc0: \<open>encoded_hp_prop_list {#} (xs @ [Hp (node x) (score x) (hps x), Hp (node y) (score y) (hps y)] @ ys) (prevs, nxts, childs, scores)\<close>
+  have enc0: \<open>encoded_hp_prop_list {#} (xs @ [Hp (node x) (score x) (hps x), Hp (node y) (score y) (hps y)] @ ys) (prevs, nxts, childs, parents, scores)\<close>
     using enc unfolding x y by (auto simp: encoded_hp_prop_list2_conc_def arr)
   then have H: \<open>fst x1= \<V> \<Longrightarrow> snd (snd x1) = None\<Longrightarrow> encoded_hp_prop_list2_conc x1 (xs @ VSIDS.link x y # ys) \<longleftrightarrow>
     encoded_hp_prop_list {#} (xs @ VSIDS.link x y # ys) (fst (snd x1))\<close> for x1
     using dist \<V> unfolding x y
     by (cases x1)
       (simp add: encoded_hp_prop_list2_conc_def)
-  have [intro!]: \<open>ch\<^sub>x \<noteq> [] \<Longrightarrow> ys \<noteq> [] \<Longrightarrow> node (hd ch\<^sub>x) \<noteq> node (hd ys)\<close>
+  have KK [intro!]: \<open>ch\<^sub>x \<noteq> [] \<Longrightarrow> ys \<noteq> [] \<Longrightarrow> node (hd ch\<^sub>x) \<noteq> node (hd ys)\<close>
     using dist2 sc' by simp
+
   show ?thesis
     unfolding hp_link_def arr prod.simps
     apply refine_vcg
@@ -744,77 +921,92 @@ proof -
         using p(1-10) p(12)[symmetric] dist2 \<V>
         apply (solves simp)
         apply (subst arg_cong2[THEN iffD1, of _ _ _ _ \<open>encoded_hp_prop_list {#}\<close>, OF _ _ encoded_hp_prop_list_link[of \<open>{#}\<close> xs \<open>node x\<close> \<open>score x\<close> \<open>hps x\<close> \<open>node y\<close> \<open>score y\<close> \<open>hps y\<close> ys
-          prevs nxts childs scores, OF enc0]])
+          prevs nxts childs parents scores, OF enc0]])
         subgoal
           using sc' p(1-10) p(12)[symmetric] dist2 \<V>
           by (simp add: x y)
         subgoal
-          using sc' p(1-10) p(12)[symmetric] dist2 \<V>
+          using sc' p(1-10) p(12)[symmetric] dist2 \<V> par
           apply (simp add: x y)
           apply (intro conjI impI)
           subgoal apply (simp add: fun_upd_idem fun_upd_twist  fun_upd_idem[of \<open>childs(parent \<mapsto> ch)\<close>] hp_set_all_def)
             apply (subst fun_upd_idem[of \<open>childs(parent \<mapsto> ch)\<close>])
-            apply auto
+            apply auto[2]
             done
           subgoal
-            apply (simp (no_asm_simp) add: hp_set_all_def hp_update_nxt_def fun_upd_idem fun_upd_twist)
+            supply [[goals_limit=1]]
+            apply (simp (no_asm_simp) add: hp_set_all_def hp_update_nxt_def fun_upd_idem fun_upd_twist
+              hp_update_prev_def
+              hp_update_parents_def)
+            apply (subst fun_upd_idem[of \<open>childs(parent \<mapsto> ch)\<close>])
+            apply (simp (no_asm_simp))
+            apply force
+            apply (subst fun_upd_twist[of _ _ parents])
+            apply force
+            apply (subst fun_upd_twist[of _ _ prevs])
+            apply force
+            apply blast
+            done
+          subgoal
+            apply (simp (no_asm_simp) add: hp_set_all_def hp_update_nxt_def fun_upd_idem fun_upd_twist
+              hp_update_prev_def)
             apply (subst fun_upd_idem[of \<open>childs(parent \<mapsto> ch)\<close>])
             apply (simp (no_asm_simp))
             apply force
             apply (subst fun_upd_idem[of \<open>nxts(parent := None)\<close>])
             apply (simp (no_asm_simp))
             apply force
-            apply blast
+            apply (simp (no_asm_simp))
             done
           subgoal
             apply (simp (no_asm_simp) add: hp_set_all_def hp_update_nxt_def fun_upd_idem fun_upd_twist
-              hp_update_prev_def)
+              hp_update_prev_def hp_update_parents_def)
             apply (subst fun_upd_idem[of \<open>childs(parent \<mapsto> ch)\<close>])
             apply (simp (no_asm_simp))
             apply force
             apply (subst fun_upd_twist[of _ _ prevs])
             apply force
-            apply blast
-            done
-          subgoal
-            apply (simp (no_asm_simp) add: hp_set_all_def hp_update_nxt_def fun_upd_idem fun_upd_twist
-              hp_update_prev_def)
-            apply (subst fun_upd_idem[of \<open>childs(parent \<mapsto> ch)\<close>])
-            apply (simp (no_asm_simp))
-            apply force
-            apply (subst fun_upd_twist[of _ _ prevs])
-            apply force
-            apply (subst fun_upd_idem[of \<open>nxts(ch := None)(parent \<mapsto> node (hd ys))\<close>])
-            apply (simp (no_asm_simp))
-            apply argo
-            apply blast
-            done
-          subgoal
-            apply (simp (no_asm_simp) add: hp_set_all_def hp_update_nxt_def fun_upd_idem fun_upd_twist
-              hp_update_prev_def)
-            apply (subst fun_upd_idem[of \<open>childs(parent \<mapsto> ch)\<close>])
-            apply (simp (no_asm_simp))
-            apply force
-            apply (subst fun_upd_twist[of _ _ prevs])
+            apply (subst fun_upd_twist[of _ _ parents])
             apply force
             apply (simp (no_asm_simp))
-            done
-          subgoal
-            apply (simp (no_asm_simp) add: hp_set_all_def hp_update_nxt_def fun_upd_idem fun_upd_twist
-              hp_update_prev_def)
-            apply (subst fun_upd_idem[of \<open>childs(parent \<mapsto> ch)\<close>])
-            apply (simp (no_asm_simp))
-            apply force
-            apply (subst fun_upd_twist[of _ _ prevs])
-            apply force
             apply (subst fun_upd_idem[of \<open>nxts(parent := None)(ch \<mapsto> node (hd ch\<^sub>x))\<close>])
             apply (simp (no_asm_simp))
+            apply force
+            apply force
+            done
+          subgoal
+            apply (simp (no_asm_simp) add: hp_set_all_def hp_update_nxt_def fun_upd_idem fun_upd_twist
+              hp_update_prev_def hp_update_parents_def)
+            apply (subst fun_upd_idem[of \<open>childs(parent \<mapsto> ch)\<close>])
+            apply (simp (no_asm_simp))
+            apply force
+            apply (subst fun_upd_twist[of _ _ prevs])
+            apply force
+            apply (simp (no_asm_simp))
+            done
+          subgoal
+            apply (simp (no_asm_simp) add: hp_set_all_def hp_update_nxt_def fun_upd_idem fun_upd_twist
+              hp_update_prev_def hp_update_parents_def)
+            apply (subst fun_upd_idem[of \<open>childs(parent \<mapsto> ch)\<close>])
+            apply (simp (no_asm_simp))
+            apply force
+            apply (subst fun_upd_twist2[of _ _ _ prevs])
+            apply (rule KK)
+            apply assumption
+            apply assumption
+            apply force
+            apply force
+            apply (subst fun_upd_twist[of _ _ \<open>prevs(ch := None)\<close>])
+            apply (rule KK[symmetric])
+            apply assumption
+            apply assumption
+            apply (subst fun_upd_twist[of _ _ \<open>parents\<close>])
             apply argo
             apply blast
             done
           subgoal
             apply (simp (no_asm_simp) add: hp_set_all_def hp_update_nxt_def fun_upd_idem fun_upd_twist
-              hp_update_prev_def)
+              hp_update_prev_def hp_update_parents_def)
             apply (subst fun_upd_idem[of \<open>childs(parent \<mapsto> ch)\<close>])
             apply (simp (no_asm_simp))
             apply force
@@ -822,13 +1014,18 @@ proof -
             apply (smt (z3) IntI Un_iff empty_iff mem_Collect_eq option.simps(9) option_hd_Some_hd)
             apply (smt (z3) IntI Un_iff empty_iff mem_Collect_eq option.simps(9) option_hd_Some_hd)
             apply (smt (z3) IntI Un_iff empty_iff mem_Collect_eq option.simps(9) option_hd_Some_hd)
-            apply (subst fun_upd_twist[of _ _ \<open>prevs(ch := None)\<close>])
+            apply (subst fun_upd_twist[of _ _ prevs])
+            apply force
+            apply (subst fun_upd_idem[of \<open>nxts\<close> \<open>node (last xs)\<close>])
             apply (smt (z3) IntI Un_iff empty_iff mem_Collect_eq option.simps(9) option_hd_Some_hd)
             apply (simp (no_asm))
+            apply (subst fun_upd_twist[of _ _ \<open>nxts\<close>])
+            apply argo
+            apply blast
             done
           subgoal
             apply (simp (no_asm_simp) add: hp_set_all_def hp_update_nxt_def fun_upd_idem fun_upd_twist
-              hp_update_prev_def)
+              hp_update_prev_def hp_update_parents_def)
             apply (subst fun_upd_idem[of \<open>childs(parent \<mapsto> ch)\<close>])
             apply (simp (no_asm_simp))
             apply force
@@ -842,6 +1039,9 @@ proof -
             apply (simp (no_asm_simp))
             apply (smt (z3) IntI Un_iff empty_iff mem_Collect_eq option.simps(9) option_hd_Some_hd)
             apply (simp (no_asm_simp))
+            apply (subst fun_upd_twist[of _ _ \<open>parents\<close>])
+            apply argo
+            apply blast
             done
           done
           apply (rule TrueI)
@@ -854,7 +1054,7 @@ proof -
         using p(1-10) p(12)[symmetric] dist2 \<V>
         apply simp
         apply (subst arg_cong2[THEN iffD1, of _ _ _ _ \<open>encoded_hp_prop_list {#}\<close>, OF _ _ encoded_hp_prop_list_link2[of \<open>{#}\<close> xs \<open>node x\<close> \<open>score x\<close> \<open>hps x\<close> \<open>node y\<close> \<open>score y\<close> \<open>hps y\<close> ys
-          prevs nxts childs scores, OF enc0]])
+          prevs nxts childs parents scores, OF enc0]])
         subgoal
           using sc' p(1-10) p(12)[symmetric] dist2 \<V>
           by (simp add: x y)
@@ -862,82 +1062,97 @@ proof -
           using sc' p(1-10) p(12)[symmetric] dist2 \<V>
           apply (simp add: x y)
           apply (intro conjI impI)
-          subgoal by (simp add: fun_upd_idem fun_upd_twist  fun_upd_idem[of \<open>childs(parent \<mapsto> ch)\<close>] hp_set_all_def)
           subgoal
-            apply (simp (no_asm_simp) add: hp_set_all_def hp_update_nxt_def fun_upd_idem fun_upd_twist)
+            by (simp add: fun_upd_idem fun_upd_twist  fun_upd_idem[of \<open>childs(parent \<mapsto> ch)\<close>] hp_set_all_def)
+          subgoal
+            apply (simp (no_asm_simp) add: hp_set_all_def hp_update_nxt_def fun_upd_idem fun_upd_twist
+              hp_update_prev_def hp_update_parents_def)
+            apply (subst fun_upd_twist[of _ _ prevs])
+            apply force
+            apply (subst fun_upd_idem[of prevs _ ])
+            apply (simp (no_asm_simp))
+            apply (subst fun_upd_twist[of _ _ prevs])
+            apply force
+            apply (subst fun_upd_twist[of _ _ parents])
+            apply force
+            apply (simp (no_asm_simp))
+            done
+          subgoal
+            apply (simp (no_asm_simp) add: hp_set_all_def hp_update_nxt_def fun_upd_idem fun_upd_twist
+              hp_update_prev_def)
+            apply (subst fun_upd_twist[of _ _ prevs])
+            apply force
+            apply (subst fun_upd_twist2[of _ _ _ nxts])
+            apply force
+            apply force
+            apply force
+            apply (subst fun_upd_idem[of \<open>nxts(ch := None)\<close>])
+            apply (simp (no_asm_simp))
+            apply (simp (no_asm_simp))
+            done
+          subgoal
+            apply (simp (no_asm_simp) add: hp_set_all_def hp_update_nxt_def fun_upd_idem fun_upd_twist
+              hp_update_prev_def hp_update_parents_def)
             apply (subst fun_upd_idem[of \<open>(nxts(node (last xs) \<mapsto> parent))\<close>])
             apply (simp (no_asm_simp))
             apply force
             apply (subst fun_upd_twist[of _ _ prevs])
             apply force
+            apply (subst fun_upd_twist2)
+            apply (smt (z3) IntI Un_iff empty_iff mem_Collect_eq option.simps(9) option_hd_Some_hd)
+            apply (smt (z3) IntI Un_iff empty_iff mem_Collect_eq option.simps(9) option_hd_Some_hd)
+            apply (smt (z3) IntI Un_iff empty_iff mem_Collect_eq option.simps(9) option_hd_Some_hd)
+            apply (subst fun_upd_twist[of _ _ parents])
+            apply (smt (z3) IntI Un_iff empty_iff mem_Collect_eq option.simps(9) option_hd_Some_hd)
             apply (subst fun_upd_twist[of _ _ nxts])
+            apply force
+            apply (subst fun_upd_twist[of _ _ \<open>(prevs(parent \<mapsto> node (last xs)))\<close>])
             apply force
             apply (simp (no_asm_simp))
             done
           subgoal
             apply (simp (no_asm_simp) add: hp_set_all_def hp_update_nxt_def fun_upd_idem fun_upd_twist
-              hp_update_prev_def)
+              hp_update_prev_def hp_update_parents_def)
             apply (subst fun_upd_idem[of \<open>prevs(parent := None)\<close>])
             apply (simp (no_asm_simp))
             apply force
+            apply (simp (no_asm_simp))
+            done
+          subgoal
+            apply (simp (no_asm_simp) add: hp_set_all_def hp_update_nxt_def fun_upd_idem fun_upd_twist
+              hp_update_prev_def hp_update_parents_def)
+            apply (subst fun_upd_twist2)
+            apply (smt (z3) IntI Un_iff empty_iff mem_Collect_eq option.simps(9) option_hd_Some_hd)
+            apply (smt (z3) IntI Un_iff empty_iff mem_Collect_eq option.simps(9) option_hd_Some_hd)
+            apply (smt (z3) IntI Un_iff empty_iff mem_Collect_eq option.simps(9) option_hd_Some_hd)
+            apply (subst fun_upd_twist[of _ _ parents])
+            apply force
+            apply (simp (no_asm_simp))
+            apply (subst fun_upd_idem[of \<open>prevs(parent := None)\<close>])
+            apply (simp (no_asm_simp))
+            apply (subst fun_upd_idem[of \<open>(prevs(parent := None))(_ \<mapsto> _)\<close>])
+            apply (simp (no_asm_simp))
+            apply (smt (z3) IntI Un_iff empty_iff mem_Collect_eq option.simps(9) option_hd_Some_hd)
             apply force
             done
           subgoal
             apply (simp (no_asm_simp) add: hp_set_all_def hp_update_nxt_def fun_upd_idem fun_upd_twist
-              hp_update_prev_def)
+              hp_update_prev_def hp_update_parents_def)
+            apply (subst fun_upd_twist[of _ _ prevs])
+            apply force
             apply (subst fun_upd_idem[of \<open>(prevs(parent \<mapsto> node (last xs)))(ch := None)\<close>])
-            apply (metis fun_upd_apply)
-            apply (subst fun_upd_twist[of _ _ prevs])
-            apply force
-            apply (subst fun_upd_twist2)
-            apply (smt (z3) IntI Un_iff empty_iff mem_Collect_eq option.simps(9) option_hd_Some_hd)
-            apply (smt (z3) IntI Un_iff empty_iff mem_Collect_eq option.simps(9) option_hd_Some_hd)
-            apply (smt (z3) IntI Un_iff empty_iff mem_Collect_eq option.simps(9) option_hd_Some_hd)
-            apply (subst fun_upd_idem[of \<open>nxts(ch := None)\<close>])
             apply (simp (no_asm_simp))
             apply (smt (z3) IntI Un_iff empty_iff mem_Collect_eq option.simps(9) option_hd_Some_hd)
-            apply (simp (no_asm_simp))
-            done
-          subgoal
-            apply (simp (no_asm_simp) add: hp_set_all_def hp_update_nxt_def fun_upd_idem fun_upd_twist
-              hp_update_prev_def)
-            apply (subst fun_upd_idem[of \<open>prevs(node (hd ch\<^sub>y) \<mapsto> ch)\<close>])
+            apply (subst fun_upd_idem[of \<open>nxts(node (last xs) \<mapsto> parent)\<close>])
             apply (simp (no_asm_simp))
             apply force
-            apply (subst fun_upd_twist[of _ _ prevs])
-            apply force
-            apply (simp (no_asm_simp))
-            done
-          subgoal
-            apply (simp (no_asm_simp) add: hp_set_all_def hp_update_nxt_def fun_upd_idem fun_upd_twist
-              hp_update_prev_def)
-            apply (subst fun_upd_twist2)
-            apply (smt (z3) IntI Un_iff empty_iff mem_Collect_eq option.simps(9) option_hd_Some_hd)
-            apply (smt (z3) IntI Un_iff empty_iff mem_Collect_eq option.simps(9) option_hd_Some_hd)
-            apply (smt (z3) IntI Un_iff empty_iff mem_Collect_eq option.simps(9) option_hd_Some_hd)
-            apply (subst fun_upd_idem[of \<open>nxts(_ := _)\<close>])
-            apply (simp (no_asm_simp))
-            apply (smt (z3) IntI Un_iff empty_iff mem_Collect_eq option.simps(9) option_hd_Some_hd)
             apply (subst fun_upd_twist[of _ _ nxts])
             apply force
             apply (simp (no_asm_simp))
             done
           subgoal
             apply (simp (no_asm_simp) add: hp_set_all_def hp_update_nxt_def fun_upd_idem fun_upd_twist
-              hp_update_prev_def)
-            apply (subst fun_upd_idem[of \<open>prevs(node (hd ch\<^sub>y) \<mapsto> ch)\<close>])
-            apply (simp (no_asm_simp))
-            apply force
-            apply (subst fun_upd_idem[of \<open>prevs(parent := None)(node (hd ch\<^sub>y) \<mapsto> ch)\<close>])
-            apply (simp (no_asm_simp))
-            apply (smt (z3) IntI Un_iff empty_iff mem_Collect_eq option.simps(9) option_hd_Some_hd)
-            apply (subst fun_upd_twist[of _ _ prevs])
-            apply force
-            apply (simp (no_asm_simp))
-            done
-          subgoal
-            apply (simp (no_asm_simp) add: hp_set_all_def hp_update_nxt_def fun_upd_idem fun_upd_twist
-              hp_update_prev_def)
+              hp_update_prev_def hp_update_parents_def)
             apply (subst fun_upd_idem[of \<open>(prevs(parent \<mapsto> node (last xs)))(ch := None)(node (hd ch\<^sub>y) \<mapsto> ch)\<close>])
             apply (simp (no_asm_simp))
             apply (smt (z3) IntI Un_iff empty_iff mem_Collect_eq option.simps(9) option_hd_Some_hd)
@@ -949,6 +1164,8 @@ proof -
             apply (simp (no_asm_simp))
             apply (smt (z3) IntI Un_iff empty_iff mem_Collect_eq option.simps(9) option_hd_Some_hd)
             apply (subst fun_upd_twist[of _ _ nxts])
+            apply force
+            apply (subst fun_upd_twist[of _ _ parents])
             apply force
             apply (simp (no_asm))
             done
@@ -1027,7 +1244,7 @@ proof -
       apply (auto simp: I_def)
       done
     then show ?thesis
-      using that pass\<^sub>1_append_even[of \<open>butlast xs\<close> \<open>[last xs]\<close>]
+      using that VSIDS.pass\<^sub>1_append_even[of \<open>butlast xs\<close> \<open>[last xs]\<close>]
       by (auto simp: I_def)
   qed
 
@@ -1153,7 +1370,7 @@ proof -
     show ?thesis
       using inv nxt le linkedn nnxts
       unfolding st
-      by (auto simp: I_def take_Suc take_nth pass\<^sub>1_append_even)
+      by (auto simp: I_def take_Suc take_nth VSIDS.pass\<^sub>1_append_even)
   qed
 
   show ?thesis
@@ -1325,9 +1542,9 @@ proof -
       by (rule I_Suc)
     subgoal for s a b \<V>' x2 x1a x2a x1b x2b x1c e linkedn linked new_leader x1d x2d x1e x2e
       by (auto simp: I_def Let_def)
-    subgoal using assms by (auto simp: I_def Let_def
+    subgoal using assms VSIDS.mset_nodes_pass\<^sub>2[of xs] by (auto simp: I_def Let_def
       encoded_hp_prop_list_conc_def encoded_hp_prop_list2_conc_def
-      split: option.split)
+      split: option.split simp del: VSIDS.mset_nodes_pass\<^sub>2)
     done
 qed
 
@@ -1367,6 +1584,7 @@ definition vsids_pop_min :: \<open>_\<close> where
       else do {
         let arr = hp_update_child (the h) None arr;
         let arr = hp_update_score (the h) None arr;
+        let arr = hp_update_parents (the j) None arr;
         arr \<leftarrow> merge_pairs (\<V>, arr, None) (the j);
         RETURN (h, arr)
       }
@@ -1388,11 +1606,12 @@ proof -
       get_min2_alt_def split: option.splits)
     subgoal using assms encoded_hp_prop_list_remove_min[of \<open>node (the h)\<close> \<open>score (the h)\<close> \<open>hps (the h)\<close> \<open>{#}\<close>
       \<open>fst (fst (snd arr))\<close> \<open>(fst o snd) (fst (snd arr))\<close> \<open>(fst o snd o snd) (fst (snd arr))\<close>
-      \<open>(snd o snd o snd) (fst (snd arr))\<close>]
+      \<open>(fst o snd o snd o snd) (fst (snd arr))\<close>
+      \<open>(snd o snd o snd o snd) (fst (snd arr))\<close>]
       by (cases \<open>the h\<close>; cases \<open>fst (snd arr)\<close>)
-       (auto simp: encoded_hp_prop_list_conc_def encoded_hp_prop_list2_conc_def
+       (auto simp: encoded_hp_prop_list_conc_def encoded_hp_prop_list2_conc_def hp_update_parents_def
         hp_update_nxt_def hp_update_score_def hp_update_child_def
-        get_min2_alt_def split: option.splits)
+        get_min2_alt_def split: option.splits if_splits)
     subgoal using assms by (cases \<open>the h\<close>) (auto simp: encoded_hp_prop_list_conc_def encoded_hp_prop_def
       get_min2_alt_def split: option.splits)
     subgoal using assms by (cases \<open>the h\<close>) (auto simp: encoded_hp_prop_list_conc_def encoded_hp_prop_def
@@ -1404,6 +1623,21 @@ proof -
     done
 qed
 
+lemma find_key_None_remove_key_ident: \<open>find_key a h = None \<Longrightarrow> remove_key a h = Some h\<close>
+  by (induction a h rule: find_key.induct)
+   (auto split: if_splits)
+
+lemma in_remove_key_in_find_keyD:
+  \<open>m' \<in># (if remove_key a h = None then {#} else {#the (remove_key a h)#}) +
+    (if find_key a h = None then {#} else {#the (find_key a h)#}) \<Longrightarrow>
+  distinct_mset (mset_nodes h) \<Longrightarrow>
+    x' \<in># mset_nodes m' \<Longrightarrow> x' \<in># mset_nodes h\<close>
+  using find_remove_mset_nodes_full[of h a \<open>the (remove_key a h)\<close> \<open>the (find_key a h)\<close>]
+    in_remove_key_in_nodes[of a h x']
+  apply (auto split: if_splits simp: find_key_None_remove_key_ident)
+  apply (metis hp_node_None_notin2 hp_node_in_find_key0)
+  by (metis union_iff)
+
 
 lemma encoded_hp_prop_list_remove_find:
   fixes h :: \<open>('a, nat) hp\<close> and a arr and hs :: \<open>('a, nat) hp multiset\<close>
@@ -1412,28 +1646,28 @@ lemma encoded_hp_prop_list_remove_find:
   defines \<open>arr\<^sub>3 \<equiv> (if hp_next a h = None then arr\<^sub>2 else hp_update_prev (node (the (hp_next a h))) (map_option node (hp_prev a h)) arr\<^sub>2)\<close>
   defines \<open>arr' \<equiv> hp_update_prev a None (hp_update_nxt a None arr\<^sub>3)\<close>
   assumes enc: \<open>encoded_hp_prop_list (add_mset h {#}) [] arr\<close>
-  shows \<open>encoded_hp_prop_list ((if VSIDS.remove_key a h = None then {#} else {#the (VSIDS.remove_key a h)#}) +
-        (if VSIDS.find_key a h = None then {#} else {#the (VSIDS.find_key a h)#})) []
+  shows \<open>encoded_hp_prop_list ((if remove_key a h = None then {#} else {#the (remove_key a h)#}) +
+        (if find_key a h = None then {#} else {#the (find_key a h)#})) []
         arr'\<close>
 proof -
-  obtain prevs nxts childs scores \<V> where
-    arr: \<open>arr = ((prevs, nxts, childs, scores))\<close> and
+  obtain prevs nxts childs parents scores \<V> where
+    arr: \<open>arr = ((prevs, nxts, childs, parents, scores))\<close> and
     dist: \<open>distinct_mset (mset_nodes h)\<close> and
     \<V>: \<open>set_mset (sum_list (map mset_nodes xs)) \<subseteq> \<V>\<close>
     by (cases arr) (use assms in \<open>auto simp: ac_simps encoded_hp_prop_list2_conc_def encoded_hp_prop_list_def
         encoded_hp_prop_def\<close>)
-  have find_key_in_nodes: \<open>VSIDS.find_key a h \<noteq> None \<Longrightarrow> node (the (VSIDS.find_key a h)) \<in># mset_nodes h\<close>
+  have find_key_in_nodes: \<open>find_key a h \<noteq> None \<Longrightarrow> node (the (find_key a h)) \<in># mset_nodes h\<close>
     by (cases \<open>a \<in># mset_nodes h\<close>)
    	 (use find_key_None_or_itself[of a h] in \<open>auto simp del: find_key_None_or_itself\<close>)
-  have in_find_key_in_nodes1: \<open>x \<in># mset_nodes y \<Longrightarrow> VSIDS.find_key a h = Some y \<Longrightarrow> x \<in># mset_nodes h\<close> for x y
+  have in_find_key_in_nodes1: \<open>x \<in># mset_nodes y \<Longrightarrow> find_key a h = Some y \<Longrightarrow> x \<in># mset_nodes h\<close> for x y
     using mset_nodes_find_key_subset[of a h]
     by auto
-  have [simp]: \<open>VSIDS.find_key a h = None \<Longrightarrow> VSIDS.remove_key a h = Some h\<close>
-    by (metis VSIDS.find_key.simps find_key_none_iff hp.exhaust_sel hp_node_None_notin2
+  have [simp]: \<open>find_key a h = None \<Longrightarrow> remove_key a h = Some h\<close>
+    by (metis find_key.simps find_key_none_iff hp.exhaust_sel hp_node_None_notin2
       hp_node_children_None_notin2 hp_node_children_simps2 option_last_Nil option_last_Some_iff(2)
       remove_key_notin_unchanged)
-  have \<open>VSIDS.remove_key a h \<noteq> None \<Longrightarrow> node (the (VSIDS.remove_key a h)) \<in># mset_nodes h\<close>
-    by (metis VSIDS.remove_key.simps get_min2.simps hp.exhaust_sel option.collapse option.distinct(2) remove_key_notin_unchanged)
+  have \<open>remove_key a h \<noteq> None \<Longrightarrow> node (the (remove_key a h)) \<in># mset_nodes h\<close>
+    by (metis remove_key.simps get_min2.simps hp.exhaust_sel option.collapse option.distinct(2) remove_key_notin_unchanged)
   then show ?thesis
     supply [[goals_limit=1]]
     using enc
@@ -1452,7 +1686,7 @@ proof -
       using hp_next_remove_key_other[of h a x'] find_key_None_or_itself[of a h]
         hp_next_find_key_itself[of h a] has_prev_still_in_remove_key[of h a]
         in_remove_key_changed[of a h]
-        hp_parent_itself[of h] VSIDS.remove_key_None_iff[of a h] find_key_head_node_iff[of h m']
+        hp_parent_itself[of h] remove_key_None_iff[of a h] find_key_head_node_iff[of h m']
       by (auto simp add:  hp_update_child_def hp_update_prev_def hp_update_nxt_def
         map_option.compositionality comp_def map_option_node_hp_next_remove_key
         split: if_splits  simp del: find_key_None_or_itself hp_parent_itself)
@@ -1464,9 +1698,9 @@ proof -
       using hp_prev_remove_key_other[of h a x'] find_key_None_or_itself[of a h]
         hp_prev_find_key_itself[of h a] has_prev_still_in_remove_key[of h a]
         in_remove_key_changed[of a h]
-        hp_parent_itself[of h] VSIDS.remove_key_None_iff[of a h] find_key_head_node_iff[of h m']
+        hp_parent_itself[of h] remove_key_None_iff[of a h] find_key_head_node_iff[of h m']
       using hp_prev_and_next_same_node[of h x' m' \<open>the (hp_next (node m') h)\<close>]
-        distinct_mset_find_node_next[of h \<open>node m'\<close> \<open>the (VSIDS.find_key (node m') h)\<close>]
+        distinct_mset_find_node_next[of h \<open>node m'\<close> \<open>the (find_key (node m') h)\<close>]
       apply (simp add:  hp_update_child_def hp_update_prev_def hp_update_nxt_def
         map_option.compositionality comp_def map_option_node_hp_prev_remove_key
         split: if_splits  del: find_key_None_or_itself hp_parent_itself)
@@ -1511,7 +1745,7 @@ proof -
       using hp_child_remove_key_other[of h a x'] find_key_None_or_itself[of a h]
         hp_next_find_key_itself[of h a] has_prev_still_in_remove_key[of h a]
         in_remove_key_changed[of a h]
-        hp_parent_itself[of h] VSIDS.remove_key_None_iff[of a h] find_key_head_node_iff[of h m']
+        hp_parent_itself[of h] remove_key_None_iff[of a h] find_key_head_node_iff[of h m']
 
       apply (simp add:
         split: if_splits(2)  del: find_key_None_or_itself hp_parent_itself)
@@ -1544,7 +1778,8 @@ proof -
         by (metis distinct_mset_mono' hp_child_hp_parent hp_parent_hp_child hp_parent_itself mset_nodes_find_key_subset option.sel option.simps(8) option_last_Nil option_last_Some_iff(2))
       subgoal
         apply auto
-        by (metis None_eq_map_option_iff distinct_mset_add distinct_mset_find_node_next hp_child_hp_parent hp_parent_hp_child hp_parent_itself option.map_sel option.sel option_hd_Nil option_hd_Some_iff(2))
+          by (metis (no_types, lifting) None_eq_map_option_iff distinct_mset_add distinct_mset_find_node_next hp_child_hp_parent hp_parent_hp_child hp_parent_itself
+            option.map_sel option.sel option_hd_Nil option_hd_Some_iff(2))
       apply metis
       apply metis
       apply metis
@@ -1567,82 +1802,115 @@ proof -
         split: if_splits  simp del: find_key_None_or_itself hp_parent_itself)
       subgoal
         using distinct_sum_next_prev_child[of h x']
-        apply (auto simp: VSIDS.remove_key_None_iff map_option_node_remove_key_iff)
+        apply (auto simp: map_option_node_remove_key_iff)
         apply (subst (asm) map_option_node_remove_key_iff)
         apply simp
         apply (meson distinct_mset_add)
-        by (auto simp: VSIDS.remove_key_None_iff)
+        by (auto simp: remove_key_None_iff)
       apply (clarsimp simp add:  hp_update_child_def hp_update_prev_def hp_update_nxt_def
           map_option.compositionality comp_def map_option_node_hp_next_remove_key
         split: if_splits  simp del: find_key_None_or_itself hp_parent_itself)
       subgoal
         using distinct_sum_next_prev_child[of h x']
-        apply (auto simp: VSIDS.remove_key_None_iff map_option_node_remove_key_iff)
+        apply (auto simp: remove_key_None_iff map_option_node_remove_key_iff)
         apply (subst (asm) map_option_node_remove_key_iff)
         apply simp
         apply (meson distinct_mset_add)
-        by (auto simp: VSIDS.remove_key_None_iff)
+        by (auto simp: remove_key_None_iff)
       apply (clarsimp simp add:  hp_update_child_def hp_update_prev_def hp_update_nxt_def
           map_option.compositionality comp_def map_option_node_hp_next_remove_key
         split: if_splits  simp del: find_key_None_or_itself hp_parent_itself)
       subgoal
         using distinct_sum_next_prev_child[of h x']
-        apply (auto simp: VSIDS.remove_key_None_iff map_option_node_remove_key_iff)
+        apply (auto simp: remove_key_None_iff map_option_node_remove_key_iff)
         apply (subst (asm) map_option_node_remove_key_iff)
         apply simp
         apply (meson distinct_mset_add)
-        by (auto simp: VSIDS.remove_key_None_iff)
+        by (auto simp: remove_key_None_iff)
       apply (clarsimp simp add:  hp_update_child_def hp_update_prev_def hp_update_nxt_def
           map_option.compositionality comp_def map_option_node_hp_next_remove_key
         split: if_splits  simp del: find_key_None_or_itself hp_parent_itself)
       subgoal
         using distinct_sum_next_prev_child[of h x']
-        apply (auto simp: VSIDS.remove_key_None_iff map_option_node_remove_key_iff)
+        apply (auto simp: remove_key_None_iff map_option_node_remove_key_iff)
         apply (subst (asm) map_option_node_remove_key_iff)
         apply simp
         apply (meson distinct_mset_add)
-        by (auto simp: VSIDS.remove_key_None_iff)
+        by (auto simp: remove_key_None_iff)
       apply (clarsimp simp add:  hp_update_child_def hp_update_prev_def hp_update_nxt_def
           map_option.compositionality comp_def map_option_node_hp_next_remove_key
         split: if_splits  simp del: find_key_None_or_itself hp_parent_itself)
       subgoal
         using distinct_sum_next_prev_child[of h x']
-        apply (auto simp: VSIDS.remove_key_None_iff map_option_node_remove_key_iff)
+        apply (auto simp: remove_key_None_iff map_option_node_remove_key_iff)
         apply (subst (asm) map_option_node_remove_key_iff)
         apply simp
         apply (meson distinct_mset_add)
-        by (auto simp: VSIDS.remove_key_None_iff)
+        by (auto simp: remove_key_None_iff)
       apply (clarsimp simp add:  hp_update_child_def hp_update_prev_def hp_update_nxt_def
           map_option.compositionality comp_def map_option_node_hp_next_remove_key
         split: if_splits  simp del: find_key_None_or_itself hp_parent_itself)
       subgoal
         using distinct_sum_next_prev_child[of h x']
-        apply (auto simp: VSIDS.remove_key_None_iff map_option_node_remove_key_iff)
+        apply (auto simp: remove_key_None_iff map_option_node_remove_key_iff)
         apply (subst (asm) map_option_node_remove_key_iff)
         apply simp
         apply (meson distinct_mset_add)
-        by (auto simp: VSIDS.remove_key_None_iff)
+        by (auto simp: remove_key_None_iff)
       apply (clarsimp simp add:  hp_update_child_def hp_update_prev_def hp_update_nxt_def
           map_option.compositionality comp_def map_option_node_hp_next_remove_key
         split: if_splits  simp del: find_key_None_or_itself hp_parent_itself)
       subgoal
         using distinct_sum_next_prev_child[of h x']
-        apply (auto simp: VSIDS.remove_key_None_iff map_option_node_remove_key_iff)
+        apply (auto simp: remove_key_None_iff map_option_node_remove_key_iff)
         apply (subst (asm) map_option_node_remove_key_iff)
         apply simp
         apply (meson distinct_mset_add)
-        by (auto simp: VSIDS.remove_key_None_iff)
+        by (auto simp: remove_key_None_iff)
       apply (clarsimp simp add:  hp_update_child_def hp_update_prev_def hp_update_nxt_def
           map_option.compositionality comp_def map_option_node_hp_next_remove_key
         split: if_splits  simp del: find_key_None_or_itself hp_parent_itself)
       subgoal
         using distinct_sum_next_prev_child[of h x']
-        apply (auto simp: VSIDS.remove_key_None_iff map_option_node_remove_key_iff)
+        apply (auto simp: remove_key_None_iff map_option_node_remove_key_iff)
         apply (subst (asm) map_option_node_remove_key_iff)
         apply simp
         apply (meson distinct_mset_add)
-        by (auto simp: VSIDS.remove_key_None_iff)
+        by (auto simp: remove_key_None_iff)
       done
+    subgoal for m' x'
+      apply (frule in_remove_key_in_find_keyD)
+      apply (solves auto)[]
+      apply (solves auto)[]
+      using hp_child_find_key[of h a x']
+        in_remove_key_in_nodes[of a h x'] in_find_key_notin_remove_key[of h a x']
+        in_find_key_in_nodes[of a h x']
+        hp_parent_hp_child[of h x'] hp_child_hp_parent[of h x']
+        hp_node_in_find_key[of h a x']
+        hp_parent_remove_key_other[of h a x']
+      unfolding assms(1-4) arr
+      using hp_score_remove_key_other[of h a x'] find_key_None_or_itself[of a h]
+        hp_next_find_key_itself[of h a] has_prev_still_in_remove_key[of h a]
+        in_remove_key_changed[of a h]
+        hp_parent_itself[of h] remove_key_None_iff[of a h] find_key_head_node_iff[of h m']
+        node_remove_key_in_mset_nodes[of a h]
+      apply (clarsimp simp add:  hp_update_child_def hp_update_prev_def hp_update_nxt_def
+          map_option.compositionality comp_def map_option_node_hp_next_remove_key hp_update_parents_def
+        split: if_splits  simp del: find_key_None_or_itself hp_parent_itself)
+      apply (intro conjI impI allI)
+      apply  (auto simp add:  hp_update_child_def hp_update_prev_def hp_update_nxt_def
+          map_option.compositionality comp_def map_option_node_hp_next_remove_key hp_update_parents_def
+        split: if_splits  simp del: find_key_None_or_itself hp_parent_itself)[]
+      apply (metis no_relative_ancestor_or_notin)
+      apply  (auto simp add:  hp_update_child_def hp_update_prev_def hp_update_nxt_def
+          map_option.compositionality comp_def map_option_node_hp_next_remove_key hp_update_parents_def
+        split: if_splits  simp del: find_key_None_or_itself hp_parent_itself)[]
+using
+        hp_parent_remove_key_other[of h a x']
+apply simp
+       find_theorems find_key hp_parent
+         apply (subst (asm) hp_parent_remove_key_other)
+sorry
     subgoal for m' x'
       using hp_child_find_key[of h a x']
         in_remove_key_in_nodes[of a h x'] in_find_key_notin_remove_key[of h a x']
@@ -1653,7 +1921,7 @@ proof -
       using hp_score_remove_key_other[of h a x'] find_key_None_or_itself[of a h]
         hp_next_find_key_itself[of h a] has_prev_still_in_remove_key[of h a]
         in_remove_key_changed[of a h]
-        hp_parent_itself[of h] VSIDS.remove_key_None_iff[of a h] find_key_head_node_iff[of h m']
+        hp_parent_itself[of h] remove_key_None_iff[of a h] find_key_head_node_iff[of h m']
         node_remove_key_in_mset_nodes[of a h]
       by (auto simp add:  hp_update_child_def hp_update_prev_def hp_update_nxt_def
           map_option.compositionality comp_def map_option_node_hp_next_remove_key
@@ -1666,8 +1934,11 @@ proof -
     by auto
     subgoal for m'
       by auto
+    subgoal for m'
+      by auto
     done
 qed
 
+term VSIDS.decrease_key
 
 end
